theories/std/opt.v
@@ -1,38 +1,86 @@
 From heap_lang Require Import
   prelude.
 From heap_lang.language Require Import
+  tactics
   notations
   proofmode.
 From heap_lang.std Require Export
   base.
 
-Notation "&None" := (
-  InjL #()
-)(only parsing
-).
-Notation "&&None" := (
-  InjLV #()
-)(only parsing
-).
-Notation "&Some" :=
-  InjR
-( only parsing
-).
-Notation "&&Some" :=
-  InjRV
-( only parsing
-).
+Implicit Types v : val.
 
-Notation "'match:' e0 'with' 'None' => e1 | 'Some' x => e2 'end'" := (
-  Match e0 <>%binder e1 x%binder e2
-)(e0, e1, x, e2 at level 200,
+Definition opt_match : val :=
+  λ: "t" "None" "Some",
+    match: "t" with
+      InjL <> =>
+        "None" #()
+    | InjR "x" =>
+        "Some" "x"
+    end.
+Notation "'match:' e0 'with' | 'None' => e1 | 'Some' x => e2 'end'" :=
+  (opt_match e0 (λ: <>, e1) (λ: x, e2))%E
+( x at level 1,
+  e0, e1, e2 at level 200,
+  format "'[hv' match:  e0  with  '/' '[' |  None  =>  '/    ' e1 ']'  '/' '[' |  Some  x  =>  '/    ' e2  ']' '/' end ']'"
+) : expr_scope.
+Notation "'match:' e0 'with' 'None' => e1 | 'Some' x => e2 'end'" :=
+  (opt_match e0 (λ: <>, e1) (λ: x, e2))%E
+( x at level 1,
+  e0, e1, e2 at level 200,
   only parsing
 ) : expr_scope.
-Notation "'match:' e0 'with' | 'None' => e1 | 'Some' x => e2 'end'" := (
-  Match e0 <>%binder e1 x%binder e2
-)(e0, e1, x, e2 at level 200,
+Notation "'match::' e0 'with' | 'None' => e1 | 'Some' x => e2 'end'" :=
+  (opt_match e0 (λ: <>, e1)%V (λ: x, e2)%V)%E
+( x at level 1,
+  e0, e1, e2 at level 200,
+  format "'[hv' match::  e0  with  '/' '[' |  None  =>  '/    ' e1 ']'  '/' '[' |  Some  x  =>  '/    ' e2  ']' '/' end ']'"
+) : expr_scope.
+Notation "'match::' e0 'with' 'None' => e1 | 'Some' x => e2 'end'" :=
+  (opt_match e0 (λ: <>, e1)%V (λ: x, e2)%V)%E
+( x at level 1,
+  e0, e1, e2 at level 200,
   only parsing
 ) : expr_scope.
+
+Definition NoneV :=
+  InjLV #().
+Notation "'&&None'" :=
+  NoneV.
+#[global] Instance pure_opt_match_None e1 x e2 :
+  PureExec True 9
+    (match:: &&None with None => e1 | Some x => e2 end)
+    e1.
+Proof.
+  solve_pure_exec.
+Qed.
+
+Definition opt_Some : val :=
+  λ: "v", InjR "v".
+Definition SomeV :=
+  InjRV.
+Notation "'&Some'" :=
+  opt_Some.
+Notation "'&&Some'" :=
+  SomeV.
+#[global] Instance pure_opt_Some v :
+  PureExec True 2
+    (&Some v)
+    (&&Some v).
+Proof.
+  solve_pure_exec.
+Qed.
+#[global] Instance pure_opt_match_Some v e1 x e2 :
+  PureExec True 9
+    (match:: &&Some v with None => e1 | Some x => e2 end)
+    (subst' x v e2).
+Proof.
+  solve_pure_exec.
+Qed.
+
+#[global] Opaque opt_match.
+#[global] Opaque NoneV.
+#[global] Opaque opt_Some.
+#[global] Opaque SomeV.
 
 Section heap_GS.
   Context `{heap_GS : !heapGS Σ}.
@@ -52,7 +100,7 @@ Section heap_GS.
     ( WP e1 {{ Φ }} ∧
       ∀ v, τ v -∗ WP subst' x v e2 {{ Φ }}
     ) -∗
-    WP match: t with None => e1 | Some x => e2 end {{ Φ }}.
+    WP match:: t with None => e1 | Some x => e2 end {{ Φ }}.
   Proof.
     iIntros "[-> | (%v & -> & #Hv)] H";
       [rewrite bi.and_elim_l | rewrite bi.and_elim_r];
